theories/Syntax/Stmt.v
@@ -29,21 +29,3 @@ Arguments Goto {_ _ _ _}.
 Arguments Return {_ _ _ _}.
 Arguments Invoke {_ _ _ _}.
 Arguments Skip {_ _ _ _}.
-
-Inductive defined {Π Ω} `{Object Π Ω} : string → t Π Ω → Prop :=
-  | defined_seq_l x s₁ s₂ : defined x s₁ → defined x (Seq s₁ s₂)
-  | defined_seq_r x s₁ s₂ : defined x s₂ → defined x (Seq s₁ s₂)
-  | defined_assign x e : defined x (Assign x e)
-  | defined_if_true x e s₁ s₂ : defined x s₁ → defined x (If e s₁ s₂)
-  | defined_if_false x e s₁ s₂ : defined x s₂ → defined x (If e s₁ s₂).
-
-(** [free x s] is provable iff variable [x] is free in statement [s] *)
-Inductive free {Π Ω} `{Object Π Ω} : string → t Π Ω → Prop :=
-  | free_seq_l x s₁ s₂ : free x s₁ → free x (Seq s₁ s₂)
-  | free_seq_r x s₁ s₂ : free x s₂ → free x (Seq s₁ s₂)
-  | free_assign x y e : Term.free x e → free x (Assign y e)
-  | free_if_guard x e s₁ s₂ : Term.free x e → free x (If e s₁ s₂)
-  | free_if_l x e s₁ s₂ : free x s₁ → free x (If e s₁ s₂)
-  | free_if_r x e s₁ s₂ : free x s₂ → free x (If e s₁ s₂)
-  | free_return x e : Term.free x e → free x (Return e).
-
